code/flink/src/main/scala-2.11/de/bbisping/coupledsim/flink/CoupledSimulationGame.scala
@@ -35,7 +35,7 @@ class CoupledSimulationGame {
         // only generate attacker nodes where there is a chance of the defender winning
         (signatures cross signatures) flatMap new FlatMapFunction[((Int, Signature), (Int, Signature)), (Action, Int, Int)] {
           def flatMap(pqSig: ((Int, Signature), (Int, Signature)),
-              out: Collector[(Action, Int, Int)]) = pqSig match {
+              out: Collector[(Action, Int, Int)]): Unit = pqSig match {
             case ((p, pSig), (q, qSig)) =>
               if (pSig.size <= qSig.size && (pSig subsetOf qSig)) {
                 out.collect((ATTACK, p, q))
@@ -46,8 +46,6 @@ class CoupledSimulationGame {
         possibleAttackerNodes
     }
     
-    //println(attackerNodes.collect())
-  
     val simulationChallenges: DataSet[((Action, Int, Int), (Action, Int, Int))]  =
       (ts.getEdgesAsTuple3() join possibleAttackerNodes) // ? 
       .where(0/*src*/).equalTo(1/*p*/) { (edge, an) =>
@@ -57,24 +55,20 @@ class CoupledSimulationGame {
     val defenderSimulationNodes: DataSet[(Action, Int, Int)] =
       ((simulationChallenges flatMap new FlatMapFunction[((Action, Int, Int), (Action, Int, Int)), (Action, Int, Int)] { 
         def flatMap(simChallenge: ((Action, Int, Int), (Action, Int, Int)),
-              out: Collector[(Action, Int, Int)]) = simChallenge match {
-          case ((_, rhs)) =>
+              out: Collector[(Action, Int, Int)]): Unit = simChallenge match {
+          case (_, rhs) =>
             out.collect(rhs)
             //out.collect((TAU, rhs._2, rhs._3))
         }
       })
       union (possibleAttackerNodes map (an => (TAU, an._2, an._3)))
       ).distinct()
-      
-  //        Seq(rhs, (TAU, rhs._2, rhs._3))
-  //      }: (((Action, Int, Int), (Action, Int, Int))) => TraversableOnce[(Action, Int, Int)]))
-  //      .distinct()
-    
+
     // only allow "real" (non-stuttering) tau-steps (because otherwise this could be used
     // by the defender to go into infinite loops and win) (we assume that tau cycles have been compressed)
-    val tauSteps = ts.getEdgesAsTuple3() filter new FilterFunction[((Int, Int, Action))] {
-      def filter(edge: ((Int, Int, Action))) = edge match {
-        case ((p0, p1, a)) => a == TAU && p0 != p1
+    val tauSteps: DataSet[(Int, Int, Action)] = ts.getEdgesAsTuple3() filter new FilterFunction[(Int, Int, Action)] {
+      def filter(edge: (Int, Int, Action)): Boolean = edge match {
+        case (p0, p1, a) => a == TAU && p0 != p1
       }
     }
     
@@ -89,7 +83,7 @@ class CoupledSimulationGame {
     val simulationAnswers: DataSet[((Action, Int, Int), (Action, Int, Int))] =
       (defenderSimulationNodes join ts.getEdgesAsTuple3())
       .where(2/*q*/,0/*a*/).equalTo(0/*src*/,2/*a*/) (new JoinFunction[(Action, Int, Int), (Int, Int, Action), ((Action, Int, Int), (Action, Int, Int))] {
-        def join(dn: (Action, Int, Int), edge: (Int, Int, Action)) = {
+        def join(dn: (Action, Int, Int), edge: (Int, Int, Action)): ((Action, Int, Int), (Action, Int, Int)) = {
           (dn, (TAU, dn._2, edge._2))
         }
       })
@@ -98,29 +92,20 @@ class CoupledSimulationGame {
     val simulationAnswerTauResolves: DataSet[((Action, Int, Int), (Action, Int, Int))] =
       (defenderSimulationNodes
           .filter(new FilterFunction[(Action, Int, Int)] {
-            def filter(challenge: (Action, Int, Int)) = challenge._1 == TAU})
+            def filter(challenge: (Action, Int, Int)): Boolean = challenge._1 == TAU})
        join attackerNodes) // ??
-      .where(1,2).equalTo(1,2)/* { dn =>
-        (dn, (ATTACK, dn._2, dn._3))//TODO: Restrict this to attacker nodes which are in the over-approximation (otherwise this may generate spurious victories for the defender!!)
-    }*/
-    
+      .where(1,2).equalTo(1,2)
+
     // every attacker node can be the entry or exit of a coupling challenge
     val couplingChallengesEntrysExits: DataSet[((Action, Int, Int), (Action, Int, Int))]  =
       (possibleAttackerNodes map (an => (an, (COUPLING, an._2, an._3)))) union // ??
       (attackerNodes map (an => ((COUPLING, an._3, an._2), an))) // ????
-//      
-//      attackerNodes flatMap new FlatMapFunction[(Action, Int, Int), ((Action, Int, Int), (Action, Int, Int))] {
-//        def flatMap(an: (Action, Int, Int), out: Collector[((Action, Int, Int), (Action, Int, Int))]) = {
-//          out.collect((an, (COUPLING, an._2, an._3)))
-//          out.collect(((COUPLING, an._3, an._2), an))// note the reversed order of p and q!!!
-//        }
-//    }
-    
+
     // during a coupling challenge, the defender may move with tau steps on the right-hand side.
     val couplingMoves: DataSet[((Action, Int, Int), (Action, Int, Int))] =
       (possibleAttackerNodes join tauSteps)
       .where(2/*q*/).equalTo(0/*src*/) (new JoinFunction[(Action, Int, Int), (Int, Int, Action), ((Action, Int, Int), (Action, Int, Int))] {
-        def join(an: (Action, Int, Int), edge: (Int, Int, Action)) = {
+        def join(an: (Action, Int, Int), edge: (Int, Int, Action)): ((Action, Int, Int), (Action, Int, Int)) = {
           ((COUPLING, an._2, an._3), (COUPLING, an._2, edge._2))
         }
     })
@@ -132,18 +117,6 @@ class CoupledSimulationGame {
       
     (gameNodes, gameMoves)
   }
-//
-//  def genAttack(pqWithSig: ((Int, Set[(Coloring.Color, Coloring.Color)]), (Int, Set[(Coloring.Color, Coloring.Color)]))) = pqWithSig match {
-//    case ((p, pSig), (q, qSig)) =>
-//      //if (pSig.size <= qSig.size && (pSig subsetOf qSig)) {
-//         (ATTACK, p, q)
-////      } else {
-////         (ATTACK, p, q)
-////      }
-//  }
-      
-    //  (Int, Set[(Coloring.Color, Coloring.Color)]), (Int, Set[(Coloring.Color, Coloring.Color)]))) => Seq[(Action, Int, Int)]
-  
   
 }
 
