code/flink/src/main/scala-2.11/de/bbisping/coupledsim/flink/SignatureRefinement.scala
@@ -1,56 +1,61 @@
 package de.bbisping.coupledsim.flink
 
-import org.apache.flink.api.scala._
-import org.apache.flink.api.scala.DataSet
+import java.lang.{Long => JavaLong}
+
+import de.bbisping.coupledsim.util.Coloring
+import org.apache.flink.api.scala.{DataSet, _}
+import org.apache.flink.api.scala.utils.DataSetUtils
 import org.apache.flink.graph.scala.Graph
 import org.apache.flink.types.NullValue
-import de.bbisping.coupledsim.util.Coloring
-import org.apache.flink.api.common.functions.FlatMapFunction
-import org.apache.flink.util.Collector
-import org.apache.flink.api.common.functions.FilterFunction
-import org.apache.flink.api.common.functions.JoinFunction
-import scala.reflect.ClassTag
-import org.apache.flink.api.common.typeinfo.TypeInformation
-import org.apache.flink.api.scala.utils.`package`.DataSetUtils
 
 
 class SignatureRefinement {
-  
-  import CoupledSimulationFlink.Action
-  
+
+  import SignatureRefinement._
+
   type Signature = Set[(Coloring.Color, Coloring.Color)]
-  
+
   def compute(
       ts: Graph[Int, NullValue, CoupledSimulationFlink.Action])
   : (DataSet[(Int, Coloring.Color)], DataSet[(Int, Set[(Coloring.Color, Coloring.Color)])]) = {
-    
-    val initialColoring: DataSet[(Int, Coloring.Color)] = ts.getVertexIds().map((_, 0))
-    
+
+    val verts = ts.getVertexIds()
+
+    val initialColoring: DataSet[(Int, Color)] = verts.map((_, Long.MinValue))
+
     val coloring = initialColoring.iterateWithTermination(CoupledSimulationFlink.MAX_ITERATIONS) { coloring =>
 
-      val oldSigs: DataSet[(Int, Int)] = coloring.map(_._2).distinct.map(s => (1,1))
-      val oldSigCount: DataSet[(Int, Int)] = oldSigs.sum(0)
+      val oldSigCount: DataSet[Tuple1[Int]] = coloring.map(_._2).distinct.map(_ => Tuple1(1)).sum(0)
       
-      val signatureEdges: DataSet[(Int, (Coloring.Color, Coloring.Color))] = ts.getEdgesAsTuple3().join(coloring).where(1).equalTo(0) {
+      val signatureEdges: DataSet[(Int, (Color, Color))] = ts.getEdgesAsTuple3().join(coloring).where(1).equalTo(0) {
         (edge, color) => (edge._1, (edge._3.toInt, color._2))
       }
-      val signatures: DataSet[(Int, Set[(Coloring.Color, Coloring.Color)])] = signatureEdges.groupBy(0).reduceGroup { g =>
-        val head = g.next()
-        (head._1, g.map(_._2).toSet + head._2)
+      val signatures: DataSet[(Int, Color)] =
+        signatureEdges.groupBy(0).reduceGroup { g =>
+          val head = g.next
+          (head._1, longHashing(g.map(_._2).toSet + head._2))
+        }
+
+      // new colors for the vertices, still keeping color for vertices without out-edges!
+      val newColoring: DataSet[(Int, Color)] = coloring.leftOuterJoin(signatures)
+        .where(0).equalTo(0) { (oldColoring, newColor) =>
+        if (newColor == null) (oldColoring._1, Long.MinValue) else newColor
       }
-      
-      val newColoring: DataSet[(Int, Coloring.Color)] = coloring.leftOuterJoin(signatures)
-        .where(0).equalTo(0) ((oldColoring, newSig) => if (newSig == null) oldColoring else (newSig._1, newSig._2.hashCode()))
-      
-      val newSigCount: DataSet[(Int, Int)] = newColoring.map(_._2).distinct.map(s => (1,1)).sum(0)
-      
+
+      val newSigCount: DataSet[Tuple1[Int]] = newColoring.map(_._2).distinct.map(_ => Tuple1(1)).sum(0)
+
       val terminationSet = (oldSigCount cross newSigCount).filter(on => on._1._1 < on._2._1)
-      
+
       (newColoring, terminationSet)
     }
-    
+
+    val compactColorIds: DataSet[(Long, Color)] = DataSetUtils(coloring.map(_._2).distinct).zipWithIndex
+    val compactColoring = (coloring join compactColorIds).where(1).equalTo(1) {
+      (vertSig, sigId) => (vertSig._1, sigId._1.toInt)
+    }
+
     // recompute the last signatures
-    val signatureEdges: DataSet[(Int, (Coloring.Color, Coloring.Color))] = ts.getEdgesAsTuple3().join(coloring).where(1).equalTo(0) {
+    val signatureEdges: DataSet[(Int, (Coloring.Color, Coloring.Color))] = ts.getEdgesAsTuple3().join(compactColoring).where(1).equalTo(0) {
       (edge, color) => (edge._1, (edge._3.toInt, color._2))
     }
     val signatures: DataSet[(Int, Set[(Coloring.Color, Coloring.Color)])] = signatureEdges.groupBy(0).reduceGroup { g =>
@@ -58,7 +63,73 @@ class SignatureRefinement {
       (head._1, g.map(_._2).toSet + head._2)
     }
     
-    (coloring, signatures)
+    (compactColoring, signatures)
   }
   
+}
+
+object SignatureRefinement {
+
+  type Color = Long
+
+  class FullSignature(entries: Set[(Coloring.Color, Coloring.Color)]) extends Ordered[FullSignature] {
+    lazy private val str = entries.mkString(",")
+
+    def compare(that: FullSignature): Int = str compare that.str
+  }
+
+
+  def longHashing(xs: TraversableOnce[Any]) = {
+    // adapted from https://github.com/scala/scala/blob/v2.12.5/src/library/scala/util/hashing/MurmurHash3.scala
+    var a, b, n = 0L
+    var c = 1L
+    xs foreach { x =>
+      val h = x.hashCode
+      a += h
+      b ^= h
+      if (h != 0) c *= h
+      n += 1
+    }
+    var h = 23L
+    h = mix(h, a)
+    h = mix(h, b)
+    h = mixLast(h, c)
+    finalizeHash(h, n)
+  }
+
+  /** Mix in a block of data into an intermediate hash value. */
+  final def mix(hash: Long, data: Long): Long = {
+    var h = mixLast(hash, data)
+    h = JavaLong.rotateLeft(h, 13)  //Integer.rotateLeft(h, 13)
+    h * 5 + 0xe6546b64
+  }
+
+  /** May optionally be used as the last mixing step. Is a little bit faster than mix,
+    *  as it does no further mixing of the resulting hash. For the last element this is not
+    *  necessary as the hash is thoroughly mixed during finalization anyway. */
+  final def mixLast(hash: Long, data: Long): Long = {
+    var k = data
+
+    k *= 0xcc9e2d51
+    k = JavaLong.rotateLeft(k, 15)
+    k *= 0x1b873593
+
+    hash ^ k
+  }
+
+  /** Finalize a hash to incorporate the length and make sure all bits avalanche. */
+  final def finalizeHash(hash: Long, length: Long): Long = avalanche(hash ^ length)
+
+  /** Force all bits of the hash to avalanche. Used for finalizing the hash. */
+  private final def avalanche(hash: Long): Long = {
+    var h = hash
+
+    h ^= h >>> 16
+    h *= 0x85ebca6b
+    h ^= h >>> 13
+    h *= 0xc2b2ae35
+    h ^= h >>> 16
+
+    h
+  }
 }
