code/flink/src/main/scala-2.11/de/bbisping/coupledsim/flink/SignatureRefinementDelta.scala
@@ -1,0 +1,141 @@
+package de.bbisping.coupledsim.flink
+
+import de.bbisping.coupledsim.flink.CoupledSimulationFlink.Action
+import de.bbisping.coupledsim.util.Coloring
+import org.apache.flink.api.common.functions.FlatMapFunction
+import org.apache.flink.api.scala.{DataSet, _}
+import org.apache.flink.api.scala.utils.DataSetUtils
+import org.apache.flink.graph.scala.Graph
+import org.apache.flink.types.NullValue
+import org.apache.flink.util.Collector
+
+/**
+  * Not yet working properly. (Because of instable hashes in graph circles)
+  */
+class SignatureRefinementDelta {
+
+  import SignatureRefinement._
+
+  type Signature = Set[(Coloring.Color, Coloring.Color)]
+
+  def compute(
+      ts: Graph[Int, NullValue, CoupledSimulationFlink.Action])
+  : (DataSet[(Int, Coloring.Color)], DataSet[(Int, Set[(Coloring.Color, Coloring.Color)])]) = {
+
+    val verts = ts.getVertexIds()
+
+    val initialColoring: DataSet[(Int, Color)] = verts.map((_, Long.MinValue))
+
+    val coloring = initialColoring.iterateDelta(initialColoring, CoupledSimulationFlink.MAX_ITERATIONS, Array(0)) { (currentColoring, lastChanges) =>
+
+      // we only have to update predecessors of changed vertices
+      val activeVertices: DataSet[Int] =
+        (lastChanges join ts.getEdgeIds() where (v => v._1) equalTo 1) { (_, edge) => println(edge._1); edge._1 }.distinct
+
+      val oldSignatures: DataSet[(Int, Color)] =
+        (activeVertices join currentColoring where (v => v) equalTo 0) { (_, oldSig) => oldSig }
+
+      // the edges originating from active vertices have to be considered to compute new signatures
+      val activeEdges: DataSet[(Int, Int, Action)] =
+        (activeVertices join ts.getEdgesAsTuple3() where (v => v) equalTo 0) { (_, edge) => edge }
+
+      val signatureEdges: DataSet[(Int, (Color, Color))] =
+        (activeEdges join currentColoring where 1 equalTo 0) { (edge, color) =>
+          (edge._1, (edge._3, color._2))
+      }
+
+      val signatureUpdates: DataSet[(Int, Color)] =
+        signatureEdges.groupBy(0).reduceGroup { g =>
+          val head = g.next
+          (head._1, longHashing(g.map(_._2).toSet + head._2))
+        }
+
+      val vertexColorComparison: DataSet[(Int, Color, Color)] =
+        (signatureUpdates join currentColoring where 0 equalTo 0) { (newSig, oldSig) =>
+          (newSig._1, newSig._2, oldSig._2)
+      }
+
+      val reallyUpdatedVertices = vertexColorComparison flatMap new FlatMapFunction[(Int, Color, Color), (Int, Color)] {
+        def flatMap(change: (Int, Color, Color),
+                    out: Collector[(Int, Color)]): Unit = change match {
+          case (id: Int, newColor: Color, oldColor: Color) =>
+            if (newColor != oldColor) {
+              println(id, oldColor, newColor)
+              out.collect((id, newColor))
+            }
+        }
+      }
+//
+//
+//      filter new FilterFunction[(Int, Color, Color)] {
+//        def filter(update: (Int, Color, Color)): Boolean = update match {
+//          case (id: Int, newColor: Color, oldColor: Color) => newColor != oldColor
+//        }
+//      }
+//
+//      val reallyUpdatedVertices = realUpdates map (change => change._1)
+
+      (reallyUpdatedVertices, reallyUpdatedVertices)
+    }
+/*
+    val coloring = initialColoring.iterateWithTermination(CoupledSimulationFlink.MAX_ITERATIONS) { coloring =>
+
+      //val oldSigMaxId: DataSet[Color] = coloring.max(1).map(_._2)
+      //val oldSigs: DataSet[(Int, Int)] = coloring.map(_._2).distinct.map(_ => (1,1))
+      val oldSigCount: DataSet[(Int, Int)] = coloring.map(_._2).distinct.map(_ => (1,1)).sum(0)
+      
+      val signatureEdges: DataSet[(Int, (Color, Color))] = ts.getEdgesAsTuple3().join(coloring).where(1).equalTo(0) {
+        (edge, color) => (edge._1, (edge._3.toInt, color._2))
+      }
+      val signatures: DataSet[(Int, Color)] =
+        signatureEdges.groupBy(0).reduceGroup { g =>
+          val head = g.next
+          (head._1, longHashing((g.map(_._2)).toSet + head._2))
+        }
+/*
+      // defragment colors (new IDs on LHS)
+      val signatureColors: DataSet[(Color, Color)] =
+        DataSetUtils(signatures.map(s => s._2).distinct).zipWithIndex
+
+      val verticesColored: DataSet[(Int, Color)] =
+        (signatures join signatureColors).where(1).equalTo(1) {
+          (vertSig, sigId) => (vertSig._1, sigId._1)
+        }*/
+
+      // new colors for the vertices, still keeping color for vertices without out-edges!
+      val newColoring: DataSet[(Int, Color)] = coloring.leftOuterJoin(signatures)
+        .where(0).equalTo(0) { (oldColoring, newColor) =>
+        if (newColor == null) (oldColoring._1, Long.MinValue) else newColor
+      }
+
+      //val newSigMaxId: DataSet[Color] = newColoring.max(1).map(_._2)
+      val newSigCount: DataSet[(Int, Int)] = newColoring.map(_._2).distinct.map(_ => (1,1)).sum(0)
+
+//      val terminationSet = (oldSigMaxId cross newSigMaxId) filter { on =>
+//        println(Console.GREEN + " {Old Count, new Count} " + on)
+//        on._1 < on._2
+//      }
+      val terminationSet = (oldSigCount cross newSigCount).filter(on => on._1._1 < on._2._1)
+
+      (newColoring, terminationSet)
+    }
+*/
+    val compactColorIds: DataSet[(Long, Color)] = DataSetUtils(coloring.map(_._2).distinct).zipWithIndex
+    val compactColoring = (coloring join compactColorIds).where(1).equalTo(1) {
+      (vertSig, sigId) => (vertSig._1, sigId._1.toInt)
+    }
+
+    // recompute the last signatures
+    val signatureEdges: DataSet[(Int, (Coloring.Color, Coloring.Color))] = ts.getEdgesAsTuple3().join(compactColoring).where(1).equalTo(0) {
+      (edge, color) => (edge._1, (edge._3.toInt, color._2))
+    }
+    val signatures: DataSet[(Int, Set[(Coloring.Color, Coloring.Color)])] = signatureEdges.groupBy(0).reduceGroup { g =>
+      val head = g.next()
+      (head._1, g.map(_._2).toSet + head._2)
+    }
+    
+    (compactColoring, signatures)
+  }
+  
+}
+
