isabelle/CS_Fixpoint_Algo_Delay.thy
@@ -1,0 +1,111 @@
+section \<open>Fixed Point Algorithm for Coupled Similarity\<close>
+
+theory CS_Fixpoint_Algo_Delay
+imports
+  Coupled_Simulation
+  Finite_Weak_Transition_Systems
+  "~~/src/HOL/Library/While_Combinator"
+  "~~/src/HOL/Library/Finite_Lattice"
+begin
+
+context lts_tau
+begin
+
+definition fp_step :: 
+  "'s rel \<Rightarrow> 's rel"
+  where
+  "fp_step R1 \<equiv> { (p,q)\<in>R1.
+    (\<forall> p' a. p \<longmapsto> a p' \<longrightarrow> 
+       (\<exists> q'. ((p',q')\<in>R1) \<and> (q \<longmapsto>^~ a q')))
+  \<and> (\<exists> q'. q \<longmapsto>*tau q' \<and> ((q',p)\<in>R1)) }"
+
+lemma mono_fp_step:
+  "mono fp_step"
+proof (rule, safe)
+  fix x y::"'s rel" and p q
+  assume
+    "x \<subseteq> y"
+    "(p, q) \<in> fp_step x"
+  thus  "(p, q) \<in> fp_step y"
+    unfolding fp_step_def
+    by (auto, blast)
+qed
+
+lemma fp_fp_step:
+  assumes
+    "R = fp_step R"
+  shows
+    "coupled_delay_simulation (\<lambda> p q. (p, q) \<in> R)"
+  using assms unfolding fp_step_def coupled_delay_simulation_def delay_simulation_def
+  by fastforce
+
+lemma gfp_fp_step_subset_gcs:
+  shows "(gfp fp_step) \<subseteq> { (p,q) . greatest_coupled_simulation p q }"
+  unfolding  gcs_eq_coupled_sim_by[symmetric] 
+proof clarify
+  fix a b
+  assume
+    "(a, b) \<in> gfp fp_step"
+  thus "a \<sqsubseteq>cs  b"
+    unfolding coupled_sim_by_eq_delay_coupled_simulation
+    using fp_fp_step mono_fp_step gfp_unfold
+    by metis
+qed
+
+lemma fp_fp_step_gcs:
+  assumes
+    "R = { (p,q) . greatest_coupled_simulation p q }"
+  shows
+    "fp_step R = R"
+  unfolding assms
+proof safe
+  fix p q
+  assume
+    "(p, q) \<in> fp_step {(x, y). greatest_coupled_simulation x y}"
+  hence "(\<forall>p' a. p \<longmapsto>a  p' \<longrightarrow> (\<exists>q'. greatest_coupled_simulation p' q' \<and> q \<longmapsto>^~ a  q')) \<and>
+    (\<exists>q'. q \<longmapsto>* tau  q' \<and> greatest_coupled_simulation q' p)"
+    unfolding fp_step_def by auto
+  hence "(\<forall>p' a. p \<longmapsto>a  p' \<longrightarrow> (\<exists>q'. greatest_coupled_simulation p' q' \<and> q \<longmapsto>^ a  q')) \<and>
+    (\<exists>q'. q \<longmapsto>* tau  q' \<and> greatest_coupled_simulation q' p)"
+    unfolding fp_step_def using weak_step_delay_implies_weak_tau by blast
+  hence "(\<forall>p' a. p \<longmapsto>a  p' \<longrightarrow> (\<exists>q'. greatest_coupled_simulation p' q' \<and> q \<longmapsto>^^ a  q')) \<and>
+    (\<exists>q'. q \<longmapsto>* tau  q' \<and> greatest_coupled_simulation q' p)" using weak_step_tau2_def by simp
+  thus "greatest_coupled_simulation p q"
+    using lts_tau.gcs by metis
+next
+  fix p q
+  assume asm:
+    "greatest_coupled_simulation p q"
+  then have "(p, q) \<in> {(x, y). greatest_coupled_simulation x y}" by blast
+  moreover from asm have \<open>\<exists> R. R p q \<and> coupled_delay_simulation R\<close>
+    unfolding gcs_eq_coupled_sim_by[symmetric] coupled_sim_by_eq_delay_coupled_simulation .
+  moreover from asm have  "(\<forall> p' a. p \<longmapsto> a p' \<longrightarrow> (\<exists> q'. (greatest_coupled_simulation p' q') \<and> (q \<longmapsto>^~ a q')))"
+    unfolding  gcs_eq_coupled_sim_by[symmetric] coupled_sim_by_eq_delay_coupled_simulation
+    by (metis coupled_delay_simulation_def delay_simulation_def)
+  moreover have  "(\<exists> q'. q \<longmapsto>*tau q' \<and> (greatest_coupled_simulation q' p))"
+    using asm gcs_is_coupled_simulation coupled_simulation_implies_coupling by blast
+  ultimately show "(p, q) \<in> fp_step {(x, y). greatest_coupled_simulation x y}"
+    unfolding fp_step_def by blast
+qed
+
+lemma gfp_fp_step_gcs: "gfp fp_step = { (p,q) . greatest_coupled_simulation p q }"
+  using fp_fp_step_gcs gfp_fp_step_subset_gcs
+  by (simp add: equalityI gfp_upperbound)
+
+end
+
+context lts_tau_finite
+begin
+lemma gfp_fp_step_while:
+  shows
+    "gfp fp_step = while (\<lambda>R. fp_step R \<noteq> R) fp_step top"
+  using gfp_while_lattice[OF mono_fp_step] finite_state_rel Finite_Set.finite_set by blast
+
+theorem coupled_sim_fp_step_while:
+  shows "while (\<lambda>R. fp_step R \<noteq> R) fp_step top = { (p,q) . greatest_coupled_simulation p q }"
+  using gfp_fp_step_while gfp_fp_step_gcs by blast
+
+end
+
+
+end
