isabelle/CS_Game_Delay.thy
@@ -1,0 +1,374 @@
+section \<open>Game for Coupled Similarity with Delay Formulation\<close>
+
+theory CS_Game_Delay
+imports
+  Coupled_Simulation
+  Simple_Game
+begin
+
+subsection \<open>The Coupled Simulation Preorder Game Using Delay Steps\<close>
+
+datatype ('s, 'a) cs_game_node =
+  AttackerNode 's 's |
+  DefenderStepNode 'a 's 's |
+  DefenderCouplingNode 's 's
+
+fun (in lts_tau) cs_game_moves ::
+  "('s, 'a) cs_game_node \<Rightarrow> ('s, 'a) cs_game_node \<Rightarrow> bool" where
+  simulation_challenge:
+    "cs_game_moves (AttackerNode p q) (DefenderStepNode a p1 q0) =
+      (p \<longmapsto> a p1 \<and> q = q0)" |
+  simulation_answer: 
+    "cs_game_moves (DefenderStepNode a p1 q0) (AttackerNode p11 q1) =
+      (q0 \<longmapsto>^~ a q1 \<and> p1 = p11)" |
+  coupling_challenge:\<comment>\<open>only difference for delay!\<close>
+    "cs_game_moves (AttackerNode p q) (DefenderCouplingNode p0 q0) =
+      (p = p0 \<and> q = q0)" |
+  coupling_answer:
+    "cs_game_moves (DefenderCouplingNode p0 q0) (AttackerNode q1 p00) =
+      (p0 = p00 \<and> q0 \<longmapsto>* tau q1)" |
+  cs_game_moves_no_step:
+    "cs_game_moves _ _ = False"
+
+fun cs_game_defender_node :: "('s, 'a) cs_game_node \<Rightarrow> bool" where
+  "cs_game_defender_node (AttackerNode _ _) = False" |
+  "cs_game_defender_node (DefenderStepNode _ _ _) = True" |
+  "cs_game_defender_node (DefenderCouplingNode _ _) = True"
+
+locale cs_game =
+  lts_tau trans \<tau> +
+  simple_game cs_game_moves cs_game_defender_node initial
+for
+  trans :: "'s \<Rightarrow> 'a \<Rightarrow> 's \<Rightarrow> bool" and
+  \<tau> :: "'a" and 
+  initial :: "('s, 'a) cs_game_node"
+begin
+
+subsection \<open>Coupled Simulation Implies Winning Strategy\<close>
+
+fun strategy_from_coupleddsim :: "('s \<Rightarrow> 's \<Rightarrow> bool) \<Rightarrow> ('s, 'a) cs_game_node strategy" where
+  "strategy_from_coupleddsim R ((DefenderStepNode a p1 q0)#play) =
+    (AttackerNode p1 (SOME q1 . R p1 q1 \<and> q0 \<longmapsto>^~ a q1))" |
+  "strategy_from_coupleddsim R ((DefenderCouplingNode p0 q0)#play) =
+    (AttackerNode (SOME q1 . R q1 p0 \<and> q0 \<longmapsto>* tau q1) p0)" |
+  "strategy_from_coupleddsim _ _ = undefined"
+
+lemma attacker_followed_by_defender:
+  assumes
+    "n0 # play \<in> plays"
+    "cs_game_defender_node n0"
+    "initial = AttackerNode p0 q0"
+  shows "\<exists> p q . hd play = AttackerNode p q \<and> cs_game_moves (AttackerNode p q) n0" "play \<noteq> []"
+proof -
+  have n0_not_init: "n0 \<noteq> initial" using assms(2,3) by auto
+  hence "cs_game_moves (hd play) n0" using assms(1)
+    by (metis list.sel(1) list.sel(3) plays.cases)
+  thus "\<exists>p q. hd play = AttackerNode p q \<and> cs_game_moves (AttackerNode p q) n0" using assms(2)
+    by (metis cs_game_defender_node.elims(2,3) local.cs_game_moves_no_step(1,2,3,7))
+  show "play \<noteq> []" using n0_not_init assms(1) plays.cases by auto
+qed
+
+lemma strategy_from_coupleddsim_retains_coupledsim:
+  assumes
+    "R p0 q0"
+    "coupled_delay_simulation R"
+    "initial = AttackerNode p0 q0"
+    "play \<in> plays_for_strategy (strategy_from_coupleddsim R)"
+  shows
+    "hd play = AttackerNode p q \<Longrightarrow> R p q"
+    "length play > 1 \<Longrightarrow> hd (tl play) = AttackerNode p q \<Longrightarrow> R p q"
+  using assms(4)
+proof (induct arbitrary: p q rule: plays_for_strategy.induct[OF assms(4)])
+  case 1
+  fix p q
+  assume "hd [initial] = AttackerNode p q"
+  hence "p = p0" "q = q0" using assms(3) by auto
+  thus "R p q" using assms(1) by simp
+next
+  case 1
+  fix p q
+  assume "1 < length [initial]"
+  hence False by auto
+  thus "R p q"  ..
+next
+  case (2 n0 play)
+  hence n0play_is_play: "n0 # play \<in> plays" using strategy_plays_subset by blast
+  fix p q
+  assume subassms:
+    "hd (strategy_from_coupleddsim R (n0 # play) # n0 # play) = AttackerNode p q"
+    "strategy_from_coupleddsim R (n0 # play) # n0 # play
+      \<in> plays_for_strategy (strategy_from_coupleddsim R)"
+  then obtain pi qi where 
+      piqi_def: "hd (play) = AttackerNode pi qi"
+        "cs_game_moves (AttackerNode pi qi) n0" "play \<noteq> []"
+    using attacker_followed_by_defender[OF n0play_is_play `cs_game_defender_node n0` assms(3)]
+    by blast
+  hence "R pi qi" using 2(1,3) by simp
+  have "(\<exists> a . n0 = (DefenderStepNode a p qi) \<and> pi \<longmapsto> a p)
+    \<or> (n0 = (DefenderCouplingNode pi qi))"
+    using piqi_def(2) 2(4,5) subassms(1)
+    by (metis cs_game_defender_node.elims(2) cs_game_moves.simps(2) list.sel(1)
+        coupling_challenge simulation_challenge)
+  thus "R p q"
+  proof safe
+    fix a
+    assume n0_def: "n0 = DefenderStepNode a p qi" "pi \<longmapsto>a p"
+    have "strategy_from_coupleddsim R (n0 # play) =
+        (AttackerNode p (SOME q1 . R p q1 \<and> qi \<longmapsto>^~ a q1))"
+      unfolding n0_def(1) by auto
+    with subassms(1) have q_def: "q = (SOME q1. R p q1 \<and> qi \<longmapsto>^~ a  q1)" by auto
+    have "\<exists> qii . R p qii \<and> qi \<longmapsto>^~ a qii"
+      using n0_def(2) `R pi qi` `coupled_delay_simulation R`
+      unfolding coupled_delay_simulation_def delay_simulation_def by blast
+    from someI_ex[OF this] show "R p q" unfolding q_def by blast
+  next
+    assume n0_def: "n0 = DefenderCouplingNode pi qi"
+    have "strategy_from_coupleddsim R (n0 # play) =
+        (AttackerNode (SOME q1 . R q1 pi \<and> qi \<longmapsto>* tau q1) pi)"
+      unfolding n0_def(1) by auto
+    with subassms(1) have qp_def: "p = (SOME q1 . R q1 pi \<and> qi \<longmapsto>* tau q1)" "q = pi" by auto
+    have "\<exists> q1 . R q1 pi \<and> qi \<longmapsto>* tau q1"
+      using n0_def `R pi qi` `coupled_delay_simulation R`
+      unfolding coupled_delay_simulation_def by blast
+    from someI_ex[OF this] show "R p q" unfolding qp_def by blast
+  qed
+next
+  case (2 n0 play)
+  fix p q
+  assume "hd (tl (strategy_from_coupleddsim R (n0 # play) # n0 # play)) = AttackerNode p q"
+  hence False using 2(4) by auto
+  thus "R p q" ..
+next
+  case (3 n1 play n1')
+  fix p q
+  assume "hd (n1' # n1 # play) = AttackerNode p q"
+  hence False using 3(4,5) unfolding player1_position_def
+    by (metis cs_game_moves_no_step(5) cs_game_defender_node.elims(3) list.sel(1))
+  thus "R p q" ..
+next
+  case (3 n1 play n1')
+  fix p q
+  assume "hd (tl (n1' # n1 # play)) = AttackerNode p q"
+  thus "R p q" using 3(1,2) by auto
+qed
+
+lemma strategy_from_coupleddsim_sound:
+  assumes
+    "R p0 q0"
+    "coupled_delay_simulation R"
+    "initial = AttackerNode p0 q0"
+  shows
+    "sound_strategy (strategy_from_coupleddsim R)"
+  unfolding sound_strategy_def
+proof clarify
+  fix n0 play
+  assume subassms:
+    "n0 # play \<in> plays_for_strategy(strategy_from_coupleddsim R)"
+    "cs_game_defender_node n0"
+  then obtain pi qi where 
+      piqi_def: "hd (play) = AttackerNode pi qi"
+        "cs_game_moves (AttackerNode pi qi) n0" "play \<noteq> []"
+    using attacker_followed_by_defender[OF _ `cs_game_defender_node n0` assms(3)]
+      strategy_plays_subset by blast
+  hence "R pi qi"
+    using strategy_from_coupleddsim_retains_coupledsim[OF assms] list.sel subassms by auto
+  have "(\<exists> a p . n0 = (DefenderStepNode a p qi) \<and> pi \<longmapsto> a p)
+    \<or> (n0 = (DefenderCouplingNode pi qi))"
+    by (metis cs_game_defender_node.elims(2)
+        coupling_challenge simulation_challenge piqi_def(2) subassms(2))
+  thus "cs_game_moves n0 (strategy_from_coupleddsim R (n0 # play))"
+  proof safe
+    fix a p
+    assume dsn:
+      "pi \<longmapsto>a  p"
+      "n0 = DefenderStepNode a p qi"
+    hence qi_spec:
+      "(strategy_from_coupleddsim R (n0 # play)) =
+        AttackerNode p (SOME q1 . R p q1 \<and> qi \<longmapsto>^~ a q1)"
+      by simp
+    then obtain qii where qii_spec:
+      "AttackerNode p (SOME q1 . R p q1 \<and> qi \<longmapsto>^~ a q1) = AttackerNode p qii" by blast
+    have "\<exists> qii . R p qii \<and> qi \<longmapsto>^~ a qii"
+      using dsn `R pi qi` `coupled_delay_simulation R`
+      unfolding coupled_delay_simulation_def delay_simulation_def  by blast
+    from someI_ex[OF this] have "R p qii \<and> qi \<longmapsto>^~ a qii" using qii_spec by blast
+    thus "cs_game_moves (DefenderStepNode a p qi)
+          (strategy_from_coupleddsim R (DefenderStepNode a p qi # play))"
+      using qi_spec qii_spec unfolding dsn(2) by auto
+  next \<comment>\<open>coupling quite analogous.\<close>
+    assume dcn:
+      "n0 = DefenderCouplingNode pi qi"
+    hence qi_spec:
+      "(strategy_from_coupleddsim R (n0 # play)) =
+      AttackerNode (SOME q1 . R q1 pi \<and> qi \<longmapsto>* tau q1) pi"
+      by simp
+    then obtain qii where qii_spec:
+      "AttackerNode (SOME q1 . R q1 pi \<and> qi \<longmapsto>* tau q1) pi = AttackerNode qii pi" by blast
+    have "\<exists> qii . R qii pi \<and> qi \<longmapsto>* tau qii"
+      using dcn `R pi qi` `coupled_delay_simulation R`
+      unfolding coupled_delay_simulation_def by blast
+    from someI_ex[OF this] have "R qii pi \<and> qi \<longmapsto>* tau qii" using qii_spec by blast
+    thus "cs_game_moves (DefenderCouplingNode pi qi)
+        (strategy_from_coupleddsim R (DefenderCouplingNode pi qi # play))"
+      using qi_spec qii_spec unfolding dcn by auto
+  qed
+qed
+
+lemma coupleddsim_implies_winning_strategy:
+  assumes
+    "R p q"
+    "coupled_delay_simulation R"
+    "initial = AttackerNode p q"
+  shows
+    "player0_winning_strategy (strategy_from_coupleddsim R)"
+  unfolding player0_winning_strategy_def
+proof (clarify)
+  fix play
+  assume subassms:
+    "play \<in> plays_for_strategy (strategy_from_coupleddsim R)"
+    "player1_wins play"
+  show "False" using subassms
+  proof (induct rule: simple_game.plays_for_strategy.induct[OF subassms(1)])
+    case 1
+    then show ?case unfolding player1_wins_def using assms(3) by auto
+  next
+    case (2 n0 play)
+    hence "\<not> cs_game_defender_node (strategy_from_coupleddsim R (n0 # play))"
+      using cs_game_moves_no_step cs_game_defender_node.elims(2) by metis
+    hence "\<not>  player1_wins (strategy_from_coupleddsim R (n0 # play) # n0 # play)"
+      unfolding player1_wins_def by auto
+    thus ?case using 2(6) by auto
+  next
+    case (3 n1 play n1')
+    then obtain p q where n1_def: "n1 = AttackerNode p q"
+      unfolding player1_position_def using cs_game_defender_node.elims(3) by blast
+    hence "R p q"
+      using strategy_from_coupleddsim_retains_coupledsim[OF assms, of "n1 # play"] 3(1) by auto
+    have "(\<exists> p1 a . n1' = (DefenderStepNode a p1 q) \<and> (p \<longmapsto> a p1))
+        \<or> n1' = (DefenderCouplingNode p q)"
+      using n1_def `cs_game_moves n1 n1'` coupling_challenge cs_game_moves_no_step(5)
+        simulation_challenge
+      by (metis cs_game_defender_node.elims(2, 3))
+    then show ?case
+    proof 
+      assume "(\<exists> p1 a . n1' = (DefenderStepNode a p1 q) \<and> (p \<longmapsto> a p1))"
+      then obtain p1 a where 
+        n1'_def: "n1' = (DefenderStepNode a p1 q)" "p \<longmapsto> a p1"
+        by blast
+      hence "\<exists> q1 . q \<longmapsto>^~ a q1" 
+        using `R p q` `coupled_delay_simulation R`
+        unfolding coupled_delay_simulation_def delay_simulation_def by blast
+      hence "\<exists> q1 . cs_game_moves (DefenderStepNode a p1 q) (AttackerNode p1 q1)"
+        by auto
+      with `player1_wins (n1' # n1 # play)` show False unfolding player1_wins_def n1'_def
+        by (metis list.sel(1))
+    next
+      assume n1'_def: "n1' = DefenderCouplingNode p q"
+      have "\<exists> q1 . q \<longmapsto>*tau q1" 
+        using `coupled_delay_simulation R` `R p q`
+        unfolding coupled_delay_simulation_def by blast
+      hence "\<exists> q1 . cs_game_moves (DefenderCouplingNode p q) (AttackerNode q1 p)"
+        by auto
+      with `player1_wins (n1' # n1 # play)` show False unfolding player1_wins_def n1'_def
+        by (metis list.sel(1))
+    qed
+  qed
+qed
+
+subsection \<open>Winning Strategy Induces Coupled Simulation\<close>
+
+lemma winning_strategy_implies_coupleddsim:
+  assumes
+    "player0_winning_strategy f"
+    "sound_strategy f"
+  defines
+    "R == \<lambda> p q . (\<exists> play \<in> plays_for_strategy f . hd play = AttackerNode p q)"
+  shows
+    "coupled_delay_simulation R"
+  unfolding coupled_delay_simulation_def delay_simulation_def
+proof safe
+  fix p q p' a
+  assume challenge:
+    "R p q"
+    "p \<longmapsto>a  p'"
+  hence game_move: "cs_game_moves (AttackerNode p q) (DefenderStepNode a p' q)" by auto
+  have "(\<exists> play \<in> plays_for_strategy f . hd play = AttackerNode p q)"
+    using challenge(1) assms by blast
+  then obtain play where
+      play_spec: "AttackerNode p q # play \<in> plays_for_strategy f"
+    by (metis list.sel(1) simple_game.plays.cases strategy_plays_subset)
+  hence interplay: "(DefenderStepNode a p' q) # AttackerNode p q # play \<in> plays_for_strategy f"
+    using game_move by (simp add: player1_position_def simple_game.plays_for_strategy.p1move)
+  hence "\<not> player1_wins ((DefenderStepNode a p' q) # AttackerNode p q # play)"
+    using assms(1) unfolding player0_winning_strategy_def by blast
+  then obtain n1 where n1_def:
+      "n1 = f (DefenderStepNode a p' q # AttackerNode p q # play)"
+      "cs_game_moves (DefenderStepNode a p' q) n1"
+    using interplay assms(2) unfolding player0_winning_strategy_def sound_strategy_def by simp
+  obtain q' where q'_spec:
+      "(AttackerNode p' q') = n1" "q \<longmapsto>^~ a q'"
+    using n1_def(2) by (cases n1, auto)
+  hence "(AttackerNode p' q') # (DefenderStepNode a p' q) # AttackerNode p q # play
+      \<in> plays_for_strategy f"
+    using interplay n1_def by (simp add: simple_game.plays_for_strategy.p0move)
+  hence "R p' q'" unfolding R_def by (meson list.sel(1))
+  thus "\<exists>q'. R p' q' \<and> q \<longmapsto>^~ a  q'" using q'_spec(2) by blast
+next
+  fix p q 
+  assume challenge:
+    "R p q"
+  hence game_move: "cs_game_moves (AttackerNode p q) (DefenderCouplingNode p q)" by auto
+  have "(\<exists> play \<in> plays_for_strategy f . hd play = AttackerNode p q)"
+    using challenge assms by blast
+  then obtain play where
+      play_spec: "AttackerNode p q # play \<in> plays_for_strategy f"
+    by (metis list.sel(1) simple_game.plays.cases strategy_plays_subset)
+  hence interplay: "(DefenderCouplingNode p q) # AttackerNode p q # play
+      \<in> plays_for_strategy f"
+    using game_move by (simp add: player1_position_def simple_game.plays_for_strategy.p1move)
+  hence "\<not> player1_wins ((DefenderCouplingNode p q) # AttackerNode p q # play)"
+    using assms(1) unfolding player0_winning_strategy_def by blast
+  then obtain n1 where n1_def:
+      "n1 = f (DefenderCouplingNode p q # AttackerNode p q # play)"
+      "cs_game_moves (DefenderCouplingNode p q) n1"
+    using interplay assms(2)
+    unfolding player0_winning_strategy_def sound_strategy_def by simp
+  obtain q' where q'_spec:
+      "(AttackerNode q' p) = n1" "q \<longmapsto>* tau q'"
+    using n1_def(2) by (cases n1, auto)
+  hence "(AttackerNode q' p) # (DefenderCouplingNode p q) # AttackerNode p q # play
+      \<in> plays_for_strategy f"
+    using interplay n1_def by (simp add: simple_game.plays_for_strategy.p0move)
+  hence "R q' p" unfolding R_def by (meson list.sel(1))
+  thus "\<exists>q'. q \<longmapsto>* tau  q' \<and> R q' p" using q'_spec(2) by blast
+qed
+
+theorem winning_strategy_iff_coupledsim:
+  assumes
+    "initial = AttackerNode p q"
+  shows 
+    "(\<exists> f . player0_winning_strategy f \<and> sound_strategy f)
+    = p \<sqsubseteq>cs q"
+proof (rule)
+  assume
+    "(\<exists>f. player0_winning_strategy f \<and> sound_strategy f)"
+  then obtain f where
+    "coupled_delay_simulation (\<lambda>p q. \<exists>play\<in>plays_for_strategy f. hd play = AttackerNode p q)"
+    using winning_strategy_implies_coupleddsim by blast
+  moreover have "(\<lambda>p q. \<exists>play\<in>plays_for_strategy f. hd play = AttackerNode p q) p q"
+    using assms plays_for_strategy.init[of f] by (meson list.sel(1))
+  ultimately show "p \<sqsubseteq>cs q"
+    unfolding coupled_sim_by_eq_delay_coupled_simulation
+    by (metis (mono_tags, lifting))
+next
+  assume
+    "p \<sqsubseteq>cs  q"
+  thus "(\<exists>f. player0_winning_strategy f \<and> sound_strategy f)"
+    unfolding coupled_sim_by_eq_delay_coupled_simulation
+    using coupleddsim_implies_winning_strategy[OF _ _ assms]
+          strategy_from_coupleddsim_sound[OF _ _ assms] by blast
+qed
+
+end
+
+end
