code/project/plugins.sbt
@@ -1,7 +1,5 @@
-addSbtPlugin("org.scala-js" % "sbt-scalajs" % "0.6.17")
+addSbtPlugin("org.scala-js" % "sbt-scalajs" % "0.6.25")
 
-addSbtPlugin("com.typesafe.sbteclipse" % "sbteclipse-plugin" % "2.5.0")
+addSbtPlugin("com.typesafe.sbt" % "sbt-less" % "1.1.2")
 
-addSbtPlugin("com.typesafe.sbt" % "sbt-less" % "1.1.0")
-
-addSbtPlugin("com.vmunier" % "sbt-web-scalajs" % "1.0.1")
+addSbtPlugin("com.vmunier" % "sbt-web-scalajs" % "1.0.8-0.6")
