isabelle/preparedoc.sh
@@ -1,8 +1,8 @@
 #!
 
 
-~/Software/Isabelle2017/bin/isabelle build -d . Coupled_Simulation
-cp -r /home/ben/.isabelle/Isabelle2017/browser_info/Unsorted/Coupled_Simulation /home/ben/Dokumente/coupledsim/isabelle/html
+~/Software/Isabelle2018/bin/isabelle build -d . Coupled_Simulation
+cp -r /home/ben/.isabelle/Isabelle2018/browser_info/Unsorted/Coupled_Simulation /home/ben/Dokumente/coupledsimulation/coupledsim/isabelle/html/Coupled_Simulation
 
 python addLinkAnchors.py 
 
